Turn 64-bit integer division and modulus by constants into multiply-high
This trick was already implemented for 32-bit integer division and modulus.  Here we extend it to the 64-bit case.

For 32-bit target processors, the runtime library must implement 64-bit multiply-high (signed and unsigned).  Tentative implementations are provided for IA32 and PowerPC, but need testing.

cfrontend/C2C.ml
@@ -251,6 +251,14 @@ let builtins_generic = {
     "__i64_sar",
         (TInt(ILongLong, []),
          [TInt(ILongLong, []); TInt(IInt, [])],
+         false);
+    "__i64_smulh",
+        (TInt(ILongLong, []),
+         [TInt(ILongLong, []); TInt(ILongLong, [])],
+         false);
+    "__i64_umulh",
+        (TInt(IULongLong, []),
+         [TInt(IULongLong, []); TInt(IULongLong, [])],
          false)
   ]
 }
