runtime/powerpc/i64_umul.s
@@ -1,0 +1,64 @@
+# *****************************************************************
+#
+#               The Compcert verified compiler
+#
+#           Xavier Leroy, INRIA Paris
+#
+# Copyright (c) 2016 Institut National de Recherche en Informatique et
+#  en Automatique.
+#
+# Redistribution and use in source and binary forms, with or without
+# modification, are permitted provided that the following conditions are met:
+#     * Redistributions of source code must retain the above copyright
+#       notice, this list of conditions and the following disclaimer.
+#     * Redistributions in binary form must reproduce the above copyright
+#       notice, this list of conditions and the following disclaimer in the
+#       documentation and/or other materials provided with the distribution.
+#     * Neither the name of the <organization> nor the
+#       names of its contributors may be used to endorse or promote products
+#       derived from this software without specific prior written permission.
+# 
+# THIS SOFTWARE IS PROVIDED BY THE COPYRIGHT HOLDERS AND CONTRIBUTORS
+# "AS IS" AND ANY EXPRESS OR IMPLIED WARRANTIES, INCLUDING, BUT NOT
+# LIMITED TO, THE IMPLIED WARRANTIES OF MERCHANTABILITY AND FITNESS FOR
+# A PARTICULAR PURPOSE ARE DISCLAIMED. IN NO EVENT SHALL <COPYRIGHT
+# HOLDER> BE LIABLE FOR ANY DIRECT, INDIRECT, INCIDENTAL, SPECIAL,
+# EXEMPLARY, OR CONSEQUENTIAL DAMAGES (INCLUDING, BUT NOT LIMITED TO,
+# PROCUREMENT OF SUBSTITUTE GOODS OR SERVICES; LOSS OF USE, DATA, OR
+# PROFITS; OR BUSINESS INTERRUPTION) HOWEVER CAUSED AND ON ANY THEORY OF
+# LIABILITY, WHETHER IN CONTRACT, STRICT LIABILITY, OR TORT (INCLUDING
+# NEGLIGENCE OR OTHERWISE) ARISING IN ANY WAY OUT OF THE USE OF THIS
+# SOFTWARE, EVEN IF ADVISED OF THE POSSIBILITY OF SUCH DAMAGE.
+#
+# *********************************************************************
+
+# Helper functions for 64-bit integer arithmetic.  PowerPC version.
+
+        .text
+
+# Unsigned multiply high
+	
+# Reference C implementation in ../c/i64_umul.c
+
+        .balign 16
+        .globl __i64_umulh
+__i64_umulh:
+     # u1 in r3; u0 in r4; v1 in r5; v0 in r6
+        mulhwu   r0, r4, r6     # k (in r0) = high((u64) u0 * (u64) v0)
+        mullw    r8, r3, r6
+        mulhwu   r7, r3, r6     # t (in r8:r7) = (u64) u1 * (u64) v0
+        addc     r0, r8, r0     # w1 (in r0) = low (t + k)
+        addze    r9, r7         # w2 (in r9) = high (t + k)
+        mullw    r8, r4, r5
+        mulhwu   r7, r4, r5     # t (in r8:r7) = (u64) u0 * (u64) v1
+        addc     r0, r8, r0     # tmp (in r0) = low (t + w1)
+        addze    r0, r7         # k (in r0) = high(t + w1)
+        mullw    r8, r3, r5
+        mulhwu   r7, r3, r5     # t (in r8:r7) = (u64) u1 * (u64) v1
+        addc     r4, r8, r9     # add w2
+        addze    r3, r7
+        addc     r4, r4, r0     # add k
+        addze    r3, r3
+        blr
+        .type __i64_umulh, @function
+        .size __i64_umulh, .-__i64_umulh
